Refactored ClightSEM.

concurrency/ClightSemantincsForMachines.v
@@ -32,23 +32,48 @@ Section ClightSEM.
   (* We might want to define this properly or
      factor the machines so we don't need events here. *)
 
-  Class ClightSEM := { CLN_evsem :> @EvSem G C;
-    CLN_msem : msem CLN_evsem = CLN_memsem;
-    Sem := CLN_evsem;
-    step_decay: forall g c m tr c' m',
+  (* This should be a version of CLN_memsem annotated with memory events. 
+     Or should we just put the empty list of events at every step? *)
+  Program Definition CLN_evsem : @EvSem G C := {| msem := CLN_memsem |}.
+  Next Obligation.
+  Admitted.
+  Next Obligation.
+  Admitted.
+  Next Obligation.
+  Admitted.
+  Next Obligation.
+  Admitted.
+  Next Obligation.
+  Admitted.
+
+  Lemma CLN_msem : msem CLN_evsem = CLN_memsem.
+  Proof. auto. Qed.
+
+  Notation Sem := CLN_evsem.
+  Lemma step_decay: forall g c m tr c' m',
       event_semantics.ev_step (Sem) g c m tr c' m' ->
-      decay m m';
-    initial_core_nomem: forall n ge m v vl q om,
-      initial_core Sem n ge m v vl = Some (q, om) -> om=None;
-    initial_core_mem_congr: forall n ge m m' v vl,
-      initial_core Sem n ge m v vl = initial_core Sem n ge m' v vl;
-    at_external_SEM_eq:
+      decay m m'.
+  Admitted.
+
+  Lemma initial_core_nomem: forall n ge m v vl q om,
+      initial_core Sem n ge m v vl = Some (q, om) -> om=None.
+  Proof.
+    simpl; intros.
+    destruct (cl_initial_core _ _ _); inv H; auto.
+  Qed.
+
+  Lemma initial_core_mem_congr: forall n ge m m' v vl,
+    initial_core Sem n ge m v vl = initial_core Sem n ge m' v vl.
+  Proof. auto. Qed.
+
+  Lemma at_external_SEM_eq:
      forall ge c m, at_external Sem ge c m =
       match c with
       | State _ _ _ => None
       | ExtCall ef args _ _ _ _ => Some (ef, args)
-      end }.
+      end.
+  Proof. auto. Qed.
 
-  Instance ClightSem {CSEM : ClightSEM} : Semantics := { semG := G; semC := C; semSem := CLN_evsem }.
+  Instance ClightSem : Semantics := { semG := G; semC := C; semSem := CLN_evsem }.
 
 End ClightSEM.
